feat: Task 2

src/Interpreter.v
@@ -14,29 +14,52 @@ Inductive interpreter_result : Type :=
     bit of auxiliary notation to hide the plumbing involved in
     repeatedly matching against optional states. *)
 
-(*
-Notation "'LETOPT' x <== e1 'IN' e2"
+
+Notation "'LetSuc' ( st , cont ) '<==' e1 'in' e2"
   := (match e1 with
-          | Some x => e2
-          | None => None
+          | Success (st,cont) => e2
+          | Fail => Fail
+          | OutOfGas => OutOfGas
        end)
 (right associativity, at level 60).
-*)
 
-(**
-  2.1. TODO: Implement ceval_step as specified. To improve readability,
-             you are strongly encouraged to define auxiliary notation.
-             See the notation LETOPT in the ImpCEval chapter.
-*)
 
 Fixpoint ceval_step (st : state) (c : com) (continuation: list (state * com)) (i : nat)
                     : interpreter_result :=
   match i with
-  | (* TODO *)
-  | (* TODO *)
+  | O => OutOfGas
+  | S i' => match c with
+    | <{ skip }> => Success (st, continuation)
+    | <{ x := y }> => Success ((x !-> aeval st y; st), continuation)
+    | <{ (c1 !! c2) ; c3 }> =>
+      LetSuc ( st' , cont' ) <== (ceval_step st c1 continuation i') in
+        (ceval_step st' c3 ((st, <{ c2; c3 }>)::cont') i')
+    | <{ c1 ; c2 }> =>
+      LetSuc (st', cont') <== (ceval_step st c1 continuation i') in
+        (ceval_step st' c2 cont' i')
+    | <{ if b then c1 else c2 end }> =>
+      if (beval st b)
+      then ceval_step st c1 continuation i'
+      else ceval_step st c2 continuation i'
+    | <{ while b do c1 end }> =>
+      if (beval st b)
+      then LetSuc (st', cont') <== (ceval_step st c1 continuation i') in
+        (ceval_step st' c cont' i')
+      else Success (st,continuation)
+    | <{ c1 !! c2 }> =>
+      (* c1 is executed first *)
+        LetSuc (st', cont') <== (ceval_step st c1 continuation i') in
+          Success (st', (st, c2) :: cont')
+    | <{ b -> c1 }> =>
+      if beval st b
+      then ceval_step st c1 continuation i'
+      else
+        match continuation with
+        | [] => Fail   
+        | (st', c') :: cont' => ceval_step st' c' cont' i' 
+        end
+    end
   end.
-
-
 
 (* Helper functions that help with running the interpreter *)
 Inductive show_result : Type :=
@@ -53,6 +76,96 @@ Definition run_interpreter (st: state) (c:com) (n:nat) :=
   end.
 
 (* Tests are provided to ensure that your interpreter is working for these examples *)
+
+Example test_dsa_1:
+  run_interpreter (X !-> 5) <{ X=5 -> X:=10 }> 5 = OK [("X", 10); ("Y", 0); ("Z", 0)].
+Proof. auto. Qed.
+
+Example test_dsa_2:
+  run_interpreter (X !-> 5) <{ X=5 -> X:=10 }> 5 = OK [("X", 10); ("Y", 0); ("Z", 0)].
+Proof. auto. Qed.
+
+Example test_dsa_3:
+  run_interpreter (X !-> 5) <{ X=10 -> X:=11 }> 5 = KO.
+Proof. auto. Qed.
+
+(* Compute *)
+(*   run_interpreter (X !-> 5) <{ *)
+(*     if true then (X := 1 !! X := 2) else skip end; *)
+(*     Y := X + 1; *)
+(*     (X = 2 -> Z := 3) *)
+(*   }> 300. *)
+(**)
+(* (* the size of the continuation to the left doesn't change, but the continuatoin is different*) *)
+(* (* Compute *) *)
+(* (*   run_interpreter (X !-> 5) <{ *) *)
+(* (*     (X:=1 !! X:=2); *) *)
+(* (*     ( *) *)
+(* (*       (X = 2 -> Z := 3); *) *)
+(* (*       (Y:=1 !! Y:=2); *) *)
+(* (*       (Y = 1 -> W := 3) *) *)
+(* (*     ) *) *)
+(* (*     ; *) *)
+(* (*     (Z := 4) *) *)
+(* (*   }> 300. *) *)
+(*   *)
+(* Compute *)
+(*   run_interpreter (X !-> 0) <{ *)
+(*     (X := 1 !! X := 2); *)
+(*     Y := X + 1; *)
+(*     X = 2 -> Z := 3 *)
+(*   }> 20. *)
+(**)
+(* Compute *)
+(*   run_interpreter (X !-> 0) <{ *)
+(*     if true then (X := 1 !! X := 2) else skip end; *)
+(*     Y := X + 1; *)
+(*     X = 2 -> Z := 3 *)
+(*   }> 20. *)
+(**)
+(* Compute *)
+(*   run_interpreter (X !-> 0) <{ *)
+(*     if true then *)
+(*       if true then (X := 1 !! X := 2) else skip end *)
+(*     else *)
+(*       skip *)
+(*     end; *)
+(*     Y := X + 1; *)
+(*     X = 2 -> Z := 3 *)
+(*   }> 10. *)
+(**)
+(* Compute *)
+(*   run_interpreter (X !-> 0) <{ *)
+(*   X := 1 !! X :=2; *)
+(*   Y := 1 !! Y :=2; *)
+(*   Z := 3; *)
+(*   Y=2 -> skip; *)
+(*   X=2 -> skip *)
+(* }> 20. *)
+(**)
+(* Compute *)
+(*   run_interpreter (X !-> 0) <{ *)
+(*   X := 1 !! X :=2; *)
+(*   W := 4; *)
+(*   Y := 1 !! Y :=2; *)
+(*   Z := 3; *)
+(*   Y=2 -> skip; *)
+(*   X=2 -> skip *)
+(* }> 20. *)
+(**)
+(* Unset Printing Notations. *)
+(* Definition a132 := (<{ *)
+(*     if true then (X := 1 !! X := 2) else skip end; *)
+(*     Y := X + 1; *)
+(*     X = 2 -> X := 3 *)
+(*   }>). *)
+(* Print a132. *)
+(* Set Printing Notations. *)
+(**)
+(* Example test_dsa_4: *)
+(*   run_interpreter (X !-> 5) <{ X:=7; X=10 -> X:=11 }> 10 = KO. *)
+(* Proof. auto. Qed. *)
+
 Example test_1: 
   run_interpreter (X !-> 5) <{skip}> 1 = OK [("X", 5); ("Y", 0); ("Z", 0)].
 Proof. auto. Qed.
@@ -104,8 +217,6 @@ Example test_11:
   = OK [("X", 0); ("Y", 5); ("Z", 0)].
 Proof. auto. Qed.
 
-
-
 (**
   2.2. TODO: Prove p1_equals_p2. Recall that p1 and p2 are defined in Imp.v
 *)
@@ -114,12 +225,59 @@ Theorem p1_equals_p2: forall st cont,
   (exists i0,
     (forall i1, i1 >= i0 -> ceval_step st p1 cont i1 =  ceval_step st p2 cont i1)).
 Proof.
-  (* TODO *)
+  intros st cont. exists 5. intros.
+  do 6 (destruct i1; try lia; auto).
 Qed.
-
 
 (**
   2.3. TODO: Prove ceval_step_more.
+*)
+(**)
+(* Lemma ceval_step_one_extra: forall i st st' c cont cont', *)
+(*   ceval_step st c cont i = Success (st', cont') -> *)
+(*   ceval_step st c cont (S i) = Success (st', cont'). *)
+(* Proof. *)
+(*   intros i. *)
+(*   destruct i. *)
+(*   - intros. simpl  in H. discriminate. *)
+(*   - intros. *)
+(*     generalize dependent st. *)
+(*     generalize dependent st'. *)
+(*     generalize dependent cont. *)
+(*     generalize dependent cont'. *)
+(*     induction c. *)
+(*     -- auto. *)
+(*     -- auto. *)
+(*     -- intros scont' scont sst' sst. intros H. *)
+(**)
+(**)
+(*   induction c. *)
+(*   (* skip *) *)
+(*   - destruct i. *)
+(*     -- simpl. intros H. discriminate. *)
+(*     -- auto.  *)
+(*   (* x := a *) *)
+(*   - destruct i. *)
+(*     -- simpl. intros H. discriminate. *)
+(*     -- auto.  *)
+(*   (* c1; c2 *) *)
+(*   - destruct i. *)
+(*     -- simpl. intros H. discriminate. *)
+(*     -- intros H. simpl. asser *)
+(*        ---   *)
+(**)
+(*   destruct i. *)
+(*   - simpl. intros H. discriminate. *)
+(*   - destruct c. *)
+(*     -- simpl. intros H. assumption. *)
+(*     -- simpl. intros H. assumption. *)
+(*     -- intros H.  *)
+(*    *)
+
+(*
+
+general idea: for each type of construct, check value of subconstruct and use
+i1's result for that
 *)
 
 Theorem ceval_step_more: forall i1 i2 st st' c cont cont',
@@ -127,5 +285,99 @@ Theorem ceval_step_more: forall i1 i2 st st' c cont cont',
   ceval_step st c cont i1 = Success (st', cont') ->
   ceval_step st c cont i2 = Success (st', cont').
 Proof.
-  (* TODO *)
+  induction i1 as [|i1 IHi1].
+  - simpl ceval_step. intros. discriminate.
+  - intros.
+    -- destruct i2 as [|i2'] eqn:Ei2.
+       --- lia.
+       --- assert (Hle: i1 <= i2') by lia. 
+           destruct c.
+           (* skip *)
+           ---- trivial.
+           (* x := a *)
+           ---- trivial.
+           (* c1;c2 *)
+           ---- destruct c1.
+                ----- simpl. simpl in H0.
+                      (* i want to apply IHi1, for that I need to show that is
+                      a success *)
+                      destruct (ceval_step st _ cont i1) eqn:Eceval.
+                      ------ destruct s. apply (IHi1 i2') in Eceval. rewrite Eceval.
+                             apply (IHi1 i2') in H0. assumption. assumption. assumption.
+                      ------ discriminate.
+                      ------ discriminate.
+                ----- simpl. simpl in H0.
+                      destruct (ceval_step st <{ x := a }> cont i1) eqn:Eceval.
+                      ------ destruct s. apply (IHi1 i2') in Eceval. rewrite Eceval.
+                             apply (IHi1 i2') in H0. assumption. assumption. assumption.
+                      ------ discriminate.
+                      ------ discriminate.
+                ----- simpl. simpl in H0.
+                      destruct (ceval_step st <{ c1_1; c1_2 }> cont i1) eqn:Eceval.
+                      ------ destruct s. apply (IHi1 i2') in Eceval. rewrite Eceval.
+                             apply (IHi1 i2') in H0. assumption. assumption. assumption.
+                      ------ discriminate.
+                      ------ discriminate.
+                ----- simpl. simpl in H0.
+                      destruct (ceval_step st <{ if b then c1_1 else c1_2 end }> cont i1) eqn:Eceval.
+                      ------ destruct s. apply (IHi1 i2') in Eceval. rewrite Eceval.
+                             apply (IHi1 i2') in H0. assumption. assumption. assumption.
+                      ------ discriminate.
+                      ------ discriminate.
+                ----- simpl. simpl in H0.
+                      destruct (ceval_step st <{ while b do c1 end }> cont i1) eqn:Eceval.
+                      ------ destruct s. apply (IHi1 i2') in Eceval. rewrite Eceval.
+                             apply (IHi1 i2') in H0. assumption. assumption. assumption.
+                      ------ discriminate.
+                      ------ discriminate.
+                ----- simpl. simpl in H0. 
+                      destruct (ceval_step st <{ c1_1 !! c1_2; c2 }> cont i1) eqn:Eceval.
+                      ------ destruct s. apply (IHi1 i2') in Eceval.
+                             destruct (ceval_step st c1_1 cont i1) eqn:Eceval2.
+                             ------- destruct s0. apply (IHi1 i2') in Eceval2. rewrite Eceval2.
+                                     apply (IHi1 i2') in H0. assumption. assumption. assumption.
+                             ------- discriminate.
+                             ------- discriminate.
+                             ------- assumption.
+                      ------ destruct (ceval_step st c1_1 cont i1) eqn:Eceval2.
+                             ------- destruct s. apply (IHi1 i2') in Eceval2. rewrite Eceval2.
+                                     apply (IHi1 i2') in H0. assumption. assumption. assumption.
+                             ------- discriminate.
+                             ------- discriminate.
+                      ------ destruct (ceval_step st c1_1 cont i1) eqn:Eceval2.
+                             ------- destruct s. apply (IHi1 i2') in Eceval2. rewrite Eceval2.
+                                     apply (IHi1 i2') in H0. assumption. assumption. assumption.
+                             ------- discriminate.
+                             ------- discriminate.
+                ----- simpl. simpl in H0.
+                      destruct (ceval_step st <{ b -> c1 }> cont i1) eqn:Eceval.
+                      ------ destruct s. apply (IHi1 i2') in Eceval. rewrite Eceval.
+                             apply (IHi1 i2') in H0. assumption. assumption. assumption.
+                      ------ discriminate.
+                      ------ discriminate.
+           (* if b then c1 else c2 end *)
+           ---- simpl. destruct (beval st b) eqn: Ebeval.
+                ----- apply IHi1. assumption. simpl in H0. rewrite Ebeval in H0. assumption.
+                ----- apply IHi1. assumption. simpl in H0. rewrite Ebeval in H0. assumption.
+           (* while b do c end *)
+           ---- simpl. simpl in H0. destruct (beval st b) eqn: Ebeval.
+                (* TODO: understand why destruct of function worked, but not the explicit call *)
+                ----- destruct ceval_step eqn: Eceval.
+                      ------ destruct s. apply (IHi1 i2') in Eceval. rewrite Eceval.
+                             apply (IHi1 i2') in H0. assumption. assumption. assumption.
+                      ------ discriminate.
+                      ------ discriminate.
+                ----- assumption.
+          (* c1 !! c2 *)
+           ---- simpl. simpl in H0. destruct ceval_step eqn: Eceval.
+                (* First command succeded *)
+                ----- destruct s. apply (IHi1 i2') in Eceval. rewrite Eceval. assumption. assumption.
+                (* First command failed/ran out of gas *)
+                ----- discriminate.
+                ----- discriminate.
+           ---- simpl. simpl in H0. destruct (beval st b).
+                ----- apply (IHi1 i2') in H0. assumption. assumption.
+                ----- destruct cont.
+                      ------ discriminate.
+                      ------ destruct p. apply (IHi1 i2') in H0. assumption. assumption.
 Qed.
